define memory instance with based on byte array, start using in in Run.v, cleanups in Run.v

src/Memory.v
@@ -1,18 +1,21 @@
+(* import List before bbv.Word, otherwise Word.combine gets shadowed and huge type class
+   inference failure messages will appear *)
+Require Import Coq.Lists.List.
 Require Import bbv.Word.
 Require Import Coq.ZArith.BinInt.
 Require Import riscv.util.Decidable.
-Require Import Coq.Lists.List.
 Require Import riscv.Utility.
+Require Import riscv.util.Monad.
 
 Class Memory(m: Set)(a: Set) := mkMemory {
-  loadByte : m -> a -> option Word8;
-  loadHalf : m -> a -> option Word16;
-  loadWord : m -> a -> option Word32;
-  loadDouble : m -> a -> option Word64;
-  storeByte : m -> a -> option Word8 -> m;
-  storeHalf : m -> a -> option Word16 -> m;
-  storeWord : m -> a -> option Word32 -> m;
-  storeDouble : m -> a -> option Word64 -> m;
+  loadByte : m -> a -> option Int8;
+  loadHalf : m -> a -> option Int16;
+  loadWord : m -> a -> option Int32;
+  loadDouble : m -> a -> option Int64;
+  storeByte : m -> a -> Int8 -> option m;
+  storeHalf : m -> a -> Int16 -> option m;
+  storeWord : m -> a -> Int32 -> option m;
+  storeDouble : m -> a -> Int64 -> option m;
 }.
 
 (* memory addresses are represented using Z because word does not restrict them enough,
@@ -42,3 +45,49 @@ End Memory.
 
 Arguments read_mem {_} _.
 Arguments write_mem {_} _ _.
+
+Definition read_byte(m: mem 8)(a: Z): option (word 8) := read_mem a m.
+Definition read_half(m: mem 8)(a: Z): option (word 16) :=
+  v0 <- read_byte m a; v1 <- read_byte m (a + 1); Return (combine v0 v1).
+Definition read_word(m: mem 8)(a: Z): option (word 32) :=
+  v0 <- read_half m a; v1 <- read_half m (a + 2); Return (combine v0 v1).
+Definition read_double(m: mem 8)(a: Z): option (word 64) :=
+  v0 <- read_word m a; v1 <- read_word m (a + 4); Return (combine v0 v1).
+
+Definition lobits(sz: nat)(w: word (sz + sz)): word sz := split1 sz sz w.
+Definition hibits(sz: nat)(w: word (sz + sz)): word sz := split2 sz sz w.
+
+Definition write_byte(m: mem 8)(a: Z)(v: word 8): option (mem 8) := write_mem a v m.
+Definition write_half(m: mem 8)(a: Z)(v: word 16): option (mem 8) :=
+  m <- write_byte m a (lobits 8 v); write_byte m a (hibits 8 v).
+Definition write_word(m: mem 8)(a: Z)(v: word 32): option (mem 8) :=
+  m <- write_half m a (lobits 16 v); write_half m a (hibits 16 v).
+Definition write_double(m: mem 8)(a: Z)(v: word 64): option (mem 8) :=
+  m <- write_word m a (lobits 32 v); write_word m a (hibits 32 v).
+
+
+Definition uwordToZ{sz: nat}(w: word sz): Z := Z.of_N (wordToN w).
+
+Definition wrapLoad{aw sz: nat}(f: mem 8 -> Z -> option (word sz))
+  (m: mem 8)(a: word aw): option (SignedWord sz) :=
+  match (f m (uwordToZ a)) with
+  | Some x => Some (mkSignedWord x)
+  | None => None
+  end.
+
+Definition wrapStore{aw sz: nat}(f: mem 8 -> Z -> word sz -> option (mem 8))
+  (m: mem 8)(a: word aw)(v: SignedWord sz): option (mem 8) :=
+  match v with
+  | mkSignedWord w => f m (uwordToZ a) w
+  end.
+
+Instance mem_is_Memory(aw: nat): Memory (mem 8) (word aw) := {|
+  loadByte   := wrapLoad read_byte;
+  loadHalf   := wrapLoad read_half;
+  loadWord   := wrapLoad read_word;
+  loadDouble := wrapLoad read_double;
+  storeByte   := wrapStore write_byte;
+  storeHalf   := wrapStore write_half;
+  storeWord   := wrapStore write_word;
+  storeDouble := wrapStore write_double;
+|}.
